# Formal Definition of a Grammar

$G = \langle V_N, V_T, P, S \rangle$

* $V_N$ : Represents the set of **nonterminal symbols**. These symbols are placeholders that can be replaced by other symbols (both terminal and nonterminal) according to the grammar rules
	* $V_N = \{S, A, B, C, D\}$
* $V_T$ : Represents the set of **terminal symbols**. These symbols are the actual characters or tokens that appear in the strings of the language being generated. Terminals cannot be replaced further
	* $V_T = \{a, b, c\}$
* $V = V_N \cup V_T$ : This is the complete set of symbols, which includes both the terminal and nonterminal symbols ($V_N$ and $V_T$)
* $S \in V_N$ : Represents a specific nonterminal symbol called the **start symbol** or **axiom**. This is the initial symbol from which the generation or derivation of strings begins
* $P \subseteq V_N^+ \times V^*$ : Represents the set of **rewriting rules** or **productions**. Each rule specifies how a nonterminal (from $V_N$) can be replaced by a sequence of symbols (which could be terminals or nonterminals from $V$)
	* $P = \{ \langle \alpha, \beta \rangle \ |\ \alpha \in V_N^+ \ \text{and} \ \beta \in V^* \}$
		* $\alpha$ : a sequence of one or more nonterminal symbols ($\alpha \in V_N^+$).
		* $\beta$ : a sequence of symbols (either terminals, nonterminals, or both, denoted as $\beta \in V^*$)
		* The production rule $\langle \alpha, \beta \rangle$ can be written as $\alpha \rightarrow \beta$ , where $\alpha$ is rewritten as $\beta$ . This emphasizes the idea of **rewriting** in the grammar
		* $P = \{S \rightarrow AB, BA \rightarrow cCD, CBS \rightarrow ab, A \rightarrow \varepsilon\}$
			* $S \rightarrow AB$ : This rule means that the nonterminal $S$ can be replaced with the nonterminal sequence $AB$
			* $BA \rightarrow cCD$ : This rule states that the nonterminal sequence $BA$ can be replaced by the sequence $cCD$. This involves both terminal ($c$) and nonterminal symbols ($C$ and $D$)
			* $CBS \rightarrow ab$ : This rule states that the nonterminal sequence $CBS$ can be replaced with the terminal string $ab$
			* $A \rightarrow \varepsilon$ : This rule specifies that the nonterminal $A$ can be replaced by the empty string (denoted by $\varepsilon$). This is known as an **epsilon production** and means that $A$ can “disappear” during the rewriting process



# Relation of Immediate Derivation "$\Rightarrow$"

* $\alpha \Rightarrow \beta \quad \alpha \in V^+, \, \beta \in V^*$ if and only if $\alpha = \alpha_1 \alpha_2 \alpha_3 \space \and \space \beta = \alpha_1 \beta_2 \alpha_3$

	* This means that a string $\alpha$ is immediately derivable to $\beta$ if and only if

	* $\alpha_1$ , $\alpha_3$ are sequences of symbols that remain unchanged in the derivation

	* $\alpha_2$ is a sequence of symbols that gets rewritten as $\beta_2$ by applying a production rule from $P$ (the set of production rules)

* **Reflexive and transitive closure** is denoted by $\Rightarrow^*$ and means “zero or more rewriting steps.” In simpler terms, this is the relation that allows for **multiple steps of derivation**, including zero steps (which means the string can remain unchanged)



## Language generated by a Grammar

* $L(G) = \{ x \in V_T^* \mid S \Rightarrow^* x \}$

	* Consist only of **terminal symbols** ($x \in V_T^*$)

	* Can be derived from the **start symbol** $S$ , possibly in several steps (denoted by \($\Rightarrow ^*$), which means “zero or more derivation steps”)

	* In simple terms, L(G) is the set of all strings that can be generated by applying the grammar rules repeatedly, starting from the start symbol S , until you reach a string that only contains terminal symbols

* Some derivations may “**get stuck**,” meaning the string has nonterminal symbols, but there are no applicable rules left to rewrite them. This results in a situation where the derivation can’t continue to produce a terminal string

* Some derivations may **never terminate**, which happens if you keep applying rules without ever reaching a terminal string. This could happen if the grammar allows for infinite recursion or loops within the rules



## A First Example

* The grammar $G_1$ is defined as: 
	* $G_1 = \langle \{S, A, B\}, \{a, b, 0\}, P, S \rangle$

* The production rules $P$ can be used: 
	* $P = \{ S \rightarrow aA, A \rightarrow aS, S \rightarrow bB, B \rightarrow bS, S \rightarrow 0 \}$

* Several examples of derivations using these rules:
	* $S \Rightarrow 0$
	* $S \Rightarrow aA \Rightarrow aaS \Rightarrow aa0$
	* $ S \Rightarrow bB \Rightarrow bbS \Rightarrow bb0 $
	* $ S \Rightarrow aA \Rightarrow aaS \Rightarrow aabB \Rightarrow aabbS \Rightarrow aabb0 $
* The language generated by the grammar $G_1$ as: 
	* $L(G_1) = \{ aa, bb \}^* \cdot 0$
